Formalizing basic CGT 3

Basics.v
@@ -1,5 +1,5 @@
 Require Import ssreflect.
-Require Import Arith List Setoid BinPos BinNat Ring Relations.
+Require Import Arith List Setoid BinPos BinNat Ring Relations Bool.
 
 (* Formalization of the notion of equivalence relation *)
 
@@ -26,35 +26,83 @@ by move: (Cl_step (IHn' _ _ _ H) (Reqv Refl (n+n') (Refl z2))). Qed.
 Inductive eq {Z} (R : relation Z) : relation Z :=
   | Cl: forall {n z1 z2}, eqv R z1 z2 n -> eq R z1 z2.
 
-Implicit Arguments Cl [[Z] [R] [n] [z1] [z2]].
+Implicit Arguments Cl [[Z] [R] [z1] [z2]].
 
 Lemma equiv_eq: forall Z R, reflexive Z R -> equiv Z (eq R).
 intros Z R Refl. rewrite /equiv /reflexive /transitive /symmetric. 
 intros; split; [| split]; intros. 
- + by move: (Cl ((Reqv Refl 0) (Refl x))).
+ + by move: (Cl 0 ((Reqv Refl 0) (Refl x))).
  + inversion H. inversion H0. subst.
    apply (eqv_plus Refl) with (n':=n) in H4.
-   rewrite plus_comm in H4. by move: (Cl (Cl_step (eqv_plus Refl n0 H1) H4)).
- + inversion H. subst. by move: (Cl (Cl_swap H0)). Qed.
+   rewrite plus_comm in H4. by move: (Cl (S(n+n0)) (Cl_step (eqv_plus Refl n0 H1) H4)).
+ + inversion H. subst. by move: (Cl (S n) (Cl_swap H0)). Qed.
 
 (* Formalization of basic combinatorial group theory *)
 
+Notation "[ a ; .. ; b ]" := (a :: .. (b :: nil) ..).
+
 Definition word (X : Type) := list (X * bool).
 
-Notation "[ a ; .. ; b ]" := (a :: .. (b :: nil) ..).
+Fixpoint invw {X: Type} (w : word X) :=
+match w with
+ nil => nil
+ | (x, f) :: ws => (invw ws) ++ [(x, negb f)]
+end.
+
+Lemma invw_app: forall X (v w : word X), invw (v ++ w) = invw w ++ invw v.
+Proof. intros X. elim => [|[x f] vs IH] w. by rewrite app_nil_l app_nil_r.
+by rewrite -app_comm_cons /= app_assoc IH. Qed.
+
+Lemma invw_involutive: forall X (w : word X), invw (invw w) = w.
+Proof. intros X. elim => [|[x f] ws IH] //=. by rewrite invw_app /= negb_involutive IH. Qed.
+
 Inductive eqg {X : Type} (P : word X -> Prop) : relation (word X) :=
  | Eq_nil  : eqg P nil nil
- | Eq_triv : forall x f, eqg P [(x, f); (x, negb f)] nil
+ | Eq_triv : forall x f w, eqg P ((x, f) :: (x, negb f) :: w) w
  | Eq_rel  : forall w, P w -> eqg P w nil
  | Eq_cons : forall e y z, eqg P y z -> eqg P (e :: y) (e :: z).
+
 Implicit Arguments Eq_rel [[X] [P] [w]].
 Implicit Arguments Eq_cons [[X] [P] [y] [z]].
 
+Lemma eqg_plus: forall {X} {P : word X -> Prop} e {y z}, eqg P y z -> eqg P (e ++ y) (e ++ z).
+Proof. move => X P. elim => [|e es IH] y z H //. rewrite -?app_comm_cons.
+by move: (Eq_cons e (IH y z H)). Qed.
+
+Corollary eqg_same: forall X (P : word X -> Prop) y, eqg P y y.
+Proof. intros. rewrite -(app_nil_r y). by move: (eqg_plus y (Eq_nil P)). Qed.
+
+Corollary eqg_reflexive: forall {X} (P : word X -> Prop), reflexive (word X) (eqg P).
+Proof. rewrite /reflexive => X P x. apply eqg_same. Qed.
+
 Definition eqgg {X} (P : word X -> Prop) := eq (@eqg X P).
 
-Lemma app_left: forall X (P : word X -> Prop) z x y, eqgg P x y -> eqgg P (z++x) (z++y).
-Proof. move => X P. elim => [|z zs H] x y //=.
-rewrite /eqgg -?app_comm_cons => [[n z1 z2 A]]. apply Eq_cons.
+Corollary eqgg_trans: forall {X} (P : word X -> Prop) {x} y {z}, 
+  eqgg P x y -> eqgg P y z -> eqgg P x z.
+Proof. rewrite /eqgg => X P x y z A B. 
+move: (equiv_eq (word X) (eqg P) (eqg_reflexive P)) => [A1 [A2 A3]]. 
+rewrite /transitive in A2. apply (A2 x y z). apply A. apply B. Qed.
+
+Lemma eqv_cons: forall {X} {P : word X -> Prop} {n} e {y z},
+ eqv (eqg P) y z n -> eqv (eqg P) (e :: y) (e :: z) n.
+Proof. intros X P. induction n; intros; inversion_clear H; subst.
+ + by move: (Cl_base (Eq_cons e H0)).
+ + apply IHn with (e:=e) in H0. by move: (Cl_swap H0).
+ + apply IHn with (e:=e) in H0. apply IHn with (e:=e) in H1.
+   by move: (Cl_step H0 H1). Qed.
+
+Corollary eqgg_plus: forall {X} {P : word X -> Prop} e {y z},
+  eqgg P y z -> eqgg P (e ++ y) (e ++ z).
+Proof. intros X P. induction e as [|e es]; intros.
+ + by move: H.
+ + rewrite -?app_comm_cons. apply IHes in H. inversion H. 
+   subst. by move: (Cl n (eqv_cons e H0)). Qed.
+
+Lemma eqg_inv: forall X (P : word X -> Prop) w, eqgg P (w ++ (invw w)) nil.
+Proof. intros X P. apply (rev_ind (fun l => eqgg P (l ++ invw l) nil)).
+ + by move: (Cl 0 (Cl_base (Eq_nil P))).
+ + move => [x f] l. rewrite invw_app /=. apply (eqgg_trans P (l ++ invw l)).
+   rewrite -app_assoc /=. by move: (Cl 0 (Cl_base (eqg_plus l (Eq_triv P x f (invw l))))). Qed.
 
 (***************************)
 
